theories/ModSem.v
@@ -655,47 +655,6 @@ Section MODSEML.
     r. eapply prop_ext. split; i; auto.
   Qed.
 
-
-  Lemma alist_permutation_find K `{Dec K} V (l0 l1: alist K V)
-        (ND: NoDup (List.map fst l0))
-        (PERM: Permutation l0 l1)
-        k
-    :
-      alist_find k l0 = alist_find k l1.
-  Proof.
-    revert ND k. induction PERM; ss.
-    { i. inv ND. destruct x. rewrite eq_rel_dec_correct. des_ifs. et. }
-    { i. inv ND. inv H3. destruct x, y. rewrite eq_rel_dec_correct. des_ifs.
-      rewrite eq_rel_dec_correct in *. des_ifs. f_equal. exfalso. eapply H2. ss. auto. }
-    { i. rewrite IHPERM1; auto. rewrite IHPERM2; auto.
-      eapply Permutation_NoDup; [|apply ND].
-      eapply Permutation_map. auto.
-    }
-  Qed.
-
-  Ltac resub :=
-    repeat multimatch goal with
-           | |- context[@ITree.trigger ?E ?R ?e] =>
-             match e with
-             | subevent _ _ => idtac
-             | _ => replace (@ITree.trigger E R e) with (trigger e) by refl
-             end
-           | |- context[@subevent _ ?F ?prf _ (?e|)%sum] =>
-             let my_tac := ltac:(fun H => replace (@subevent _ F prf _ (e|)%sum) with (@subevent _ F _ _ e) by H) in
-             match (type of e) with
-             | (_ +' _) _ => my_tac ltac:(destruct e; refl)
-             | _ => my_tac ltac:(refl)
-             end
-           | |- context[@subevent _ ?F ?prf _ (|?e)%sum] =>
-             let my_tac := ltac:(fun H => replace (@subevent _ F prf _ (|e)%sum) with (@subevent _ F _ _ e) by H) in
-             match (type of e) with
-             | (_ +' _) _ => my_tac ltac:(destruct e; refl)
-             | _ => my_tac ltac:(refl)
-             end
-           | |- context[ITree.trigger (@subevent _ ?F ?prf _ (resum ?a ?b ?e))] =>
-             replace (ITree.trigger (@subevent _ F prf _ (resum a b e))) with (ITree.trigger (@subevent _ F _ _ e)) by refl
-           end.
-
   Theorem add_comm
           ms0 ms1 (P0 P1: Prop) (IMPL: P1 -> P0)
           (WF: wf (add ms1 ms0))
